

Formula Sheet—Calculus I

Derivatives of basic elementary functions:

$$(a^x)' = a^x \ln a \quad (e^x)' = e^x \quad (\log_a x)' = \frac{1}{x \ln a} \quad (\ln x)' = \frac{1}{x} \quad (x^a)' = ax^{a-1}$$

$$(\cot x)' = -\frac{1}{\sin^2 x} \quad (\tan x)' = \frac{1}{\cos^2 x} \quad (\cos x)' = -\sin x \quad (\sin x)' = \cos x$$

$$(\operatorname{arccot} x)' = -\frac{1}{1+x^2} \quad (\arctan x)' = \frac{1}{1+x^2} \quad (\arccos x)' = -\frac{1}{\sqrt{1-x^2}} \quad (\arcsin x)' = \frac{1}{\sqrt{1-x^2}}$$

$$(\cosh x)' = \sinh x \quad (\sinh x)' = \cosh x$$

Indefinite Integrals:

$$\int x^a dx = \frac{x^{a+1}}{a+1} + C, \quad (a \neq -1)$$

$$\int \frac{dx}{x} = \ln|x| + C$$

$$\int \sin x dx = -\cos x + C$$

$$\int \cos x dx = \sin x + C$$

$$\int \frac{dx}{\cos^2 x} = \tan x + C$$

$$\int \frac{dx}{\sin^2 x} = -\cot x + C$$

$$\int a^x dx = \frac{a^x}{\ln a} + C$$

$$\int e^x dx = e^x + C$$

$$\int \frac{dx}{1+x^2} = \arctan x + C$$

$$\int \frac{dx}{a^2+x^2} = \frac{1}{a} \arctan \frac{x}{a} + C$$

$$\int \frac{dx}{\sqrt{1-x^2}} = \arcsin x + C$$

$$\int \frac{dx}{\sqrt{a^2-x^2}} = \arcsin \frac{x}{a} + C$$

$$\int \frac{dx}{\sqrt{x^2+a^2}} = \ln|x + \sqrt{x^2+a^2}| + C$$

$$\int \frac{dx}{\sqrt{x^2-a^2}} = \ln|x + \sqrt{x^2-a^2}| + C$$

$$\int \frac{dx}{1-x^2} = \frac{1}{2} \ln \left| \frac{1+x}{1-x} \right| + C$$

$$\int \frac{dx}{a^2-x^2} = \frac{1}{2a} \ln \left| \frac{a+x}{a-x} \right| + C$$

$$\int \sinh x dx = \cosh x + C$$

$$\int \cosh x dx = \sinh x + C$$

(Trigonometric identities on next page)

Trigonometric Identities:

$$\sin(x + y) = \sin x \cos y + \sin y \cos x$$

$$\cos(x + y) = \cos x \cos y - \sin x \sin y$$

$$\tan(x + y) = \frac{\tan x + \tan y}{1 - \tan x \tan y}$$

$$\sin 2x = 2 \sin x \cos x$$

$$\begin{aligned}\cos 2x &= \cos^2 x - \sin^2 x \\ &= 1 - 2 \sin^2 x \\ &= 2 \cos^2 x - 1\end{aligned}$$

$$\tan 2x = \frac{2 \tan x}{1 - \tan^2 x}$$

$$\sin x + \sin y = 2 \sin \frac{x + y}{2} \cos \frac{x - y}{2}$$

$$\sin x - \sin y = 2 \sin \frac{x - y}{2} \cos \frac{x + y}{2}$$

$$\cos x + \cos y = 2 \cos \frac{x + y}{2} \cos \frac{x - y}{2}$$

$$\cos x - \cos y = -2 \sin \frac{x + y}{2} \sin \frac{x - y}{2}$$